% Copyright Â© 2013 Edward O'Callaghan. All Rights Reserved.

\section{Variables} % (fold)
\label{sec:variables}

In $\lcal$ all names are local to the definitions. In the
function $\lambda x.x$ we say that $x$ is \emph{bound}
since its occurrence in the body of the definition is
preceded by $\lambda x$. A name that is not preceded by a
$\lambda$ is said to be a \emph{free variable}.

%
\subsection{Free}

Formally we define a \emph{free} variable in the following
way:

\begin{defn}[Free Variable]
	We say that a variable $<name>$ is \emph{free} in an
	expression if one of the following cases holds:
	\begin{itemize}
		\item $<name>$ is free in $<name>$.
		\item $<name>$ is free in $\lambda <name'>.<exp>$
			if the identifier $<name> \neq <name'>$ and
			$<name>$ is free in $<exp>$.
		\item $<name>$ is free in $\textbf{E}_1 \textbf{E}_2$
			if $<name>$ is free in $\textbf{E}_1$ or free in
			$\textbf{E}_2$.
	\end{itemize}
\end{defn}

\begin{exmp}
	Consider the expression,
	\[
		(\lambda x.x)(\lambda y.yx).
	\]
	Then the $x$ in the body of the first expression from the left is
	bound to the first $\lambda$ and the $y$ in the body of the second
	expression is bound to the second $\lambda$ and the $x$ is said to
	be \emph{free}.
\end{exmp}

\begin{rem}
	Variables with the same name in different $\lambda$-expressions are
	independent. That is, $x$ is independent in the second expression
	from the $x$ in the first expression of $(\lambda x.x)(\lambda y.yx)$.
\end{rem}

%
\subsection{Bound}

Formally we define a \emph{bound} variable in the following
way:

\begin{defn}
	We say that a variable $<name>$ is \emph{bound} in an
	expression if one of the following cases hold:
	\begin{itemize}
		\item $<name>$ is bound in $\lambda <name'>.<exp>$
			if the identifier $<name>=<name'>$ or if
			$<name>$ is bound in $<exp>$.
		\item $<name>$ is bound in $\textbf{E}_1 \textbf{E}_2$
			if $<name>$ is bound in $\textbf{E}_1$ or if it is
			bound in $\textbf{E}_2$.
	\end{itemize}
\end{defn}
