% Copyright Â© 2012 Edward O'Callaghan. All Rights Reserved.

\documentclass[10pt, oneside, reqno]{amsart}

\usepackage{../../texstyle}
	
\title{Proofs}                               % Document Title
\author{Edward O'Callaghan}
\date{}                                      % Activate to display a given date or no date

\begin{document}
\maketitle \tableofcontents \clearpage

\section{Coefficient of determination (Proof)} % (fold)
\label{sec:proofone}
Given that:
\begin{defn}[total sum of squares]
	$ SS_{total} = \sum_{i=1}^{n} (y_i - \bar{y})^2 $
\end{defn}

\begin{defn}[regression sum of squares]
	$ SS_{reg} = \sum_{i=1}^{n} (\hat{y_i} - \bar{y})^2 $
\end{defn}

\begin{defn}[residual sum of squares]
	$ SS_{res} = \sum_{i=1}^{n} (y_{i} - \hat{y_{i}})^2 $
\end{defn}


\begin{prob}[Show that:]
	$ SS_{total} = SS_{reg} + SS_{res} $
\end{prob}

A direct proof is given:
\begin{proof}
\begin{align*}
 \sum_{i} (y_i - \bar{y})^2 & = \sum_{i} (\hat{y_i} - \bar{y})^2 + \sum_{i} (y_i - \hat{y_i})^2
 \\
 & = \sum_{i} ( \underbrace{ \hat{y_i} - \bar{y} }_{a} )^2 + ( \underbrace{ y_i - \hat{y_i} }_{b} )^2
 \tag{and recall that $a^2 + b^2 = (a+b)^2 - 2ab$}
 \\
 & = \sum_{i} (y_i - \bar{y})^2 - 2 \underbrace{ \sum_{i} (\hat{y_i} - \bar{y})(y_i - \hat{y_i})}_{\text{show this } = 0}
 \intertext{and so,}
 \implies \sum_{i} (\hat{y_i} - \bar{y})(y_i - \hat{y_i}) & \underset{\uparrow}{=}
 \sum_{i} ( \cancel{\bar{y}} + b_1 (x_i - \bar{x}) - \cancel{\bar{y}})(y_i - \bar{y} - b_1 (x_i - \bar{x}))
 \\
 & \text{by, } \hat{y_i} = b_0 + b_1 x_i = (\bar{y} -b_1 \bar{x}) + b_1 x_i = \bar{y} + b_1(x_i - \bar{x}) % FIXME: make this a bit more clear.. (multi-line)
 \\
 & = b_1 \sum_{i} (x_i - \bar{x}) [ y_i - \bar{y} - b_1 (x_i - \bar{x}) ]
 \\
 & = b_1 \left[ S_{xy} - b_1 S_{xx} \right]
 \\
 & = b_1 \left[ S_{xy} - \frac{S_{xy}}{\cancel{S_{xx}}} . \cancel{S_{xx}} \right] = 0 \qedhere
\end{align*}
\end{proof}

\end{document}% End of document.
